reflex case stadies/RevolvingDoor/RevolvingDoor_VC5.thy
@@ -103,48 +103,56 @@ next
     qed
   qed
 next
+  have prems:"extra3 st0" using assms extraInv_def by simp
   show "extra3 st_final"
-  proof (simp only:extra3_def; rule allI; rule impI)
-    fix s1
-    assume prems:"toEnvP s1 \<and>
-            substate s1 st_final \<and>
-            getPstate s1 ''Controller'' = ''rotating''"
-    then show "\<exists>s2 s3.
-             toEnvP s2 \<and>
-             toEnvP s3 \<and>
-             substate s2 s3 \<and>
-             substate s3 s1 \<and>
-             toEnvNum s2 s3 = 1 \<and>
-             (getPstate s2 ''Controller'' = ''motionless'' \<and>
-              getVarBool s3 ''user'' \<or>
-              getPstate s2 ''Controller'' = ''suspended'') \<and>
-             \<not> getVarBool s3 ''pressure'' \<and>
-             (\<forall>s4. toEnvP s4 \<and> substate s3 s4 \<and> substate s4 s1 \<longrightarrow>
-                   getPstate s4 ''Controller'' = ''rotating'')"
-    proof - 
-      have "extra3 st0" using assms extraInv_def by auto
-      then obtain 1:"(\<forall> s1. 
-                toEnvP s1 \<and> 
-                substate s1 st0 \<and> 
-                getPstate s1 ''Controller'' = ''rotating'' \<longrightarrow>
-                  (\<exists> s2 s3. 
-                    toEnvP s2 \<and> 
-                    toEnvP s3 \<and> 
-                    substate s2 s3 \<and> 
-                    substate s3 s1 \<and> 
-                    toEnvNum s2 s3 = 1 \<and> 
-                    (getPstate s2 ''Controller'' = ''motionless'' \<and> 
-                      getVarBool s3 ''user'' \<or>
-                      getPstate s2 ''Controller'' = ''suspended'') \<and> 
-                    \<not> getVarBool s3 ''pressure'' \<and>
-                    (\<forall> s4. 
-                      toEnvP s4 \<and> 
-                      substate s3 s4 \<and> 
-                      substate s4 s1 \<longrightarrow> 
-                        getPstate s4 ''Controller'' = ''rotating'')))" using extra3_def by auto
-      have 2:"substate st0 st_final" using assms substate_refl by auto
-      then show ?thesis using 1 assms prems extraInv_def extra3_def substate_refl substate_trans by sorry
-    qed
+  proof -
+    have 0:"toEnvP st0 \<and> toEnvP st_final \<and> st0 = predEnv st_final" using assms extraInv_def by auto
+    moreover have "P6_predEnv extra3_A extra3_B extra3_C st0" using assms extraInv_def extra3 P6_bridge by auto
+    moreover have "(AB_comb_before extra3_A (BC_to_BP4 extra3_B extra3_C)) st_final st_final"
+    proof -
+      have 1:"toEnvP st0 \<and> substate st0 st0 \<and> getPstate st0 ''Controller'' = ''rotating''" 
+        using assms extraInv_def substate_refl by auto
+      then obtain s2 s3 where
+       o1:"toEnvP s2 \<and> 
+        toEnvP s3 \<and> 
+        substate s2 s3 \<and> 
+        substate s3 st0 \<and> 
+        toEnvNum s2 s3 = 1 \<and>
+        (getPstate s2 ''Controller'' = ''motionless'' \<and>
+        getVarBool s3 ''user'' \<or>
+        getPstate s2 ''Controller'' = ''suspended'') \<and>
+        \<not> getVarBool s3 ''pressure'' \<and>
+        (\<forall>s4. toEnvP s4 \<and> substate s3 s4 \<and> substate s4 st0 \<longrightarrow>
+                getPstate s4 ''Controller'' = ''rotating'')" using extra3_def prems by blast
+      have 2:"substate st0 st_final" using calculation(1) predEnv_substate by auto
+      then have 3:"substate s3 st_final" using o1 substate_trans by blast
+      define subA where "subA \<equiv> (\<lambda>x. substate s3 x \<longrightarrow> getPstate x ''Controller'' = ''rotating'')"
+      then have "P1 subA st0" using P1_def o1 SMT.verit_bool_simplify(4) by auto
+      moreover have "subA st_final" using assms subA_def by auto
+      ultimately have "P1 subA st_final" using 0 P1_lemma by auto
+      then have 4:"(\<forall>s4. toEnvP s4 \<and> substate s3 s4 \<and> substate s4 st_final \<longrightarrow>
+                getPstate s4 ''Controller'' = ''rotating'')" using P1_def subA_def by auto
+      have 5:"s2 = predEnv s3"using o1 toEnvNum_predEnv by auto
+      have 6:"s2\<noteq>emptyState" using o1 by auto
+      have "(\<exists>s2.
+                  toEnvP s2 \<and> 
+                  substate s2 st_final \<and> 
+                  ((getPstate (predEnv s2) ''Controller'' = ''motionless'' \<and>
+                  getVarBool s2 ''user'' \<or>
+                  getPstate (predEnv s2) ''Controller'' = ''suspended'') \<and>
+                  \<not> getVarBool s2 ''pressure'') \<and>
+                  (predEnv s2) \<noteq>emptyState \<and>
+                  (\<forall>s3. toEnvP s3 \<and> substate s2 s3 \<and> substate s3 st_final \<longrightarrow>
+                          getPstate s3 ''Controller'' = ''rotating''))" using o1 3 4 5 6 by blast
+      then show ?thesis
+        apply (simp only:AB_comb_before_def BC_to_BP4_def extra3_A_def extra3_B_def extra3_C_def) 
+        using predEnvP_or_emptyState by blast 
+      qed
+      moreover have "(\<forall>x. toEnvP x \<and> substate x st_final \<and> extra3_A st_final x \<and> \<not> extra3_A st0 x \<longrightarrow> 
+          (\<exists>y. toEnvP y \<and> substate y x \<and> substate y st_final \<and> (BC_to_BP4 extra3_B extra3_C) x y))" using assms extraInv_def extra3_def BC_to_BP4_def extra3_A_def extra3_B_def extra3_C_def
+        by (smt (verit, best)) 
+      ultimately have "P6_predEnv extra3_A extra3_B extra3_C st_final" using P6_lemma by auto
+      thus ?thesis using P6_bridge extra3 by auto
   qed
 next
   show "extra6 st_final"
@@ -212,13 +220,13 @@ next
   show "R1 st_final"
   proof -
     have "toEnvP st0 \<and> toEnvP st_final \<and> st0 = predEnv st_final" using assms inv1_def extraInv_def by auto
-    moreover have "P2_predEnv R1_A2 st0" using R1_A2 assms inv1_def by auto
+    moreover have "P2_1_cons R1_A2 st0" using R1_A2 assms inv1_def by auto
     moreover have "R1_A2 st_final st0"
     proof -
       have "getPstate st_final ''Controller'' = ''rotating''" using assms by auto
       thus ?thesis using extra extraInv_def extraRotatingOut_def calculation(1) R1_A2_def substate_refl by auto
     qed
-    ultimately show ?thesis using two_pos_cond_cons_exp A2_R1 by auto
+    ultimately show ?thesis using P2_1_lemma A2_R1 by auto
   qed
 qed
 
@@ -239,44 +247,15 @@ next
   show "R2 st_final"
   proof -
     have "toEnvP st0 \<and> toEnvP st_final \<and> st0 = predEnv st_final" using assms inv2_def extraInv_def by auto
-    moreover have "P2_predEnv R2_A2 st0" using R2_A2 assms inv2_def by auto
+    moreover have "P2_1_cons R2_A2 st0" using R2_A2 assms inv2_def by auto
     moreover have "R2_A2 st_final st0" using assms R2_A2_def by auto
-    ultimately show ?thesis using two_pos_cond_cons_exp A2_R2 by auto
+    ultimately show ?thesis using P2_1_lemma A2_R2 by auto
   qed
 qed
-(*
-proof(simp only: inv2_def; rule conjI)
-  show "extraInv st_final" using assms extra inv2_def by auto
-next
-  show "R2 st_final"
-  proof(simp only: R2_def; rule conjI)
-    show "toEnvP st_final" using assms by auto
-  next
-    show "R2_sub1 st_final"
-    proof -
-       define inv2_Q1 where "inv2_Q1 = inv2_Q2 st_final"
-        have "toEnvP st0 \<and> toEnvP st_final \<and> st0=predEnv st_final" using assms inv2_def extraInv_def  by auto
-        moreover have "P2 inv2_Q2 st0" using assms P2_inv2_Q2_st0 by auto
-        moreover have "inv2_Q1 st_final" 
-        proof (simp only : inv2_Q1_def inv2_Q2_def;intro impI)
-          assume "toEnvNum st_final st_final = 1 \<and>
-                  getVarBool st_final ''rotation'' \<and>
-                  getVarBool st_final ''user'' \<and> 
-                  \<not> getVarBool st_final ''pressure''"
-          then show "getVarBool st_final ''rotation''" by (simp add: toEnvNum_id)
-        qed
-        moreover have "P1 inv2_Q1 st0" 
-          apply (simp only:P1_def inv2_Q1_def inv2_Q2_def;rule allI) 
-          using assms inv2_def extraInv_def extraRotatingOut_def
-        by (smt  calculation(1) char.inject getVarBool.simps(2) getVarBool.simps(3) getVarBool.simps(8) list.inject predEnv_substate substate_trans toEnvNum_predEnv)
-        ultimately have "P2 inv2_Q2 st_final" using inv2_Q1_def two_pos_cond_exp by auto
-        thus ?thesis using assms P2_inv2_Q2_eq_R2 R2_def by auto
-    qed
-  qed
-qed
-*)
+
+
 lemma
- assumes base_inv:"(inv st0)"
+ assumes base_inv:"(inv6 st0)"
  and st1:"(st1=(setVarBool st0 ''pressure'' pressure))"
  and st2:"(st2=(setVarBool st1 ''user'' user))"
  and st2_Controller_state:"(getPstate st2 ''Controller'')=''rotating''"
@@ -285,5 +264,91 @@ lemma
  and st3:"(st3=(reset st2 ''Controller''))"
  and st4:"(st4=(toEnv st3))"
  and st_final:"(st_final=st4)"
-shows "(inv st_final)"
+shows "(inv6 st_final)"
+proof(simp only: inv6_def; rule conjI)
+  show "extraInv st_final" using assms extra inv6_def by auto
+next
+  have extra:"extraInv st_final" using assms extra inv6_def by auto
+  show "R6 st_final"
+  proof -
+    have 0:"toEnvP st0 \<and> toEnvP st_final \<and> st0 = predEnv st_final" using assms R6_def inv6_def by auto
+    moreover have "P1 R6_A st0" using assms inv6_def R6_A by auto
+    moreover have "R6_A st_final" 
+      using R6_A_def assms inv6_def extraInv_def extraSuspendedOut_def extraMotionlessOut_def extraControllerStates_def extraRotatingOut_def local.extra substate_refl
+      by (smt (verit)) 
+    ultimately have "P1 R6_A st_final" using P1_lemma by blast
+    thus ?thesis using A_R6 0 by auto
+  qed
+qed
+
+lemma
+ assumes base_inv:"(inv4 st0)"
+ and st1:"(st1=(setVarBool st0 ''pressure'' pressure))"
+ and st2:"(st2=(setVarBool st1 ''user'' user))"
+ and st2_Controller_state:"(getPstate st2 ''Controller'')=''rotating''"
+ and st2_if5:"(getVarBool st2 ''pressure'')=False"
+ and st2_if6:"(getVarBool st2 ''user'')=True"
+ and st3:"(st3=(reset st2 ''Controller''))"
+ and st4:"(st4=(toEnv st3))"
+ and st_final:"(st_final=st4)"
+shows "(inv4 st_final)"
+proof(simp only: inv4_def; rule conjI)
+  show "extraInv st_final" using assms extra inv4_def by auto
+next
+  have extra:"extraInv st_final" using assms extra inv4_def by auto
+  show "R4_full st_final"
+  proof -
+    define inv4_A1 where "inv4_A1 = p_2_3_conpred R4_A3 st_final"
+    moreover have 0:"toEnvP st0 \<and> toEnvP st_final \<and> st0 = predEnv st_final" using assms R4_full_def inv4_def by auto
+    moreover have "P3_cons R4_A3 st0" using assms inv4_def R4_A3 R4_def by auto
+    moreover have "P1 inv4_A1 st0"
+    proof (simp only: P1_def inv4_A1_def p_2_3_conpred_def R4_A3_def SMT.verit_bool_simplify(4);rule allI; rule impI)
+      fix x
+      assume prem:"(toEnvP x \<and> substate x st0) \<and>
+               toEnvNum x st_final < 10 \<and>
+               getVarBool (predEnv x) ''rotation'' \<and>
+               getVarBool x ''pressure''"
+      then have 1:"substate x st0 \<and> substate st0 st_final \<and> substate (predEnv x) st0 \<and> substate (predEnv x) x" using 0 predEnv_substate prem substate_trans by blast 
+      then have 2: "toEnvNum st0 st_final = 1" using assms calculation(2) predEnv_toEnvNum by blast
+      then have 3:"toEnvNum x st0 < 9" using prem assms toEnvNum3
+        by (metis "1" add_less_imp_less_right numeral_plus_one semiring_norm(5) semiring_norm(8))
+      have 4:"toEnvP (predEnv x) \<and> toEnvNum (predEnv x) x =1" using predEnv_substate predEnv_toEnvNum predEnvP_or_emptyState prem by force
+      then have 5:"toEnvNum (predEnv x) st0 <10" using 1 2 predEnv_substate toEnvNum3 predEnv_toEnvNum prem predEnvP_or_emptyState by force 
+      have 6:"extra6 st0" using assms inv4_def extraInv_def by auto
+      have 7:"getPstate st0 ''Controller'' = ''rotating''" using assms by auto
+      have 8:"getPstate (predEnv x) ''Controller'' = ''rotating''"
+        using 1 4 prem base_inv inv4_def extraInv_def extraControllerStates_def extraMotionlessOut_def extraRotatingOut_def extraSuspendedOut_def
+        by meson
+      have 9:"R4_full st0" using assms inv4_def by auto
+      consider (a) "getVarBool x ''pressure''" | (b) "\<not>getVarBool x ''pressure''" by auto
+      then have "\<not>getVarBool x ''pressure''"
+      proof (cases)
+        case a
+        have "toEnvP (predEnv x) \<and> toEnvP x \<and> toEnvP st0 \<and> 
+                substate (predEnv x) x \<and> substate x st0 \<and> substate st0 st0 \<and>
+                toEnvNum (predEnv x) x = 1 \<and> toEnvNum x st0 <10 \<and>
+                getVarBool (predEnv x) ''rotation'' \<and> getVarBool x ''pressure''" 
+          using 1 4 3 prem base_inv inv4_def extraInv_def substate_refl predEnv_toEnvNum 2 9 
+          by simp
+        then have "getVarBool st0 ''brake''" using 9 R4_full_def a  by auto
+        then have "getPstate st0 ''Controller'' = ''suspended''" 
+          using base_inv inv4_def extraInv_def extra extraControllerStates_def extraMotionlessOut_def extraRotatingOut_def extraSuspendedOut_def substate_refl by blast
+        then show ?thesis using 7 by auto
+      next
+        case b
+        then show ?thesis by auto
+      qed
+      thus "getVarBool st_final ''brake''" using prem by auto
+    qed
+    moreover have "inv4_A1 st_final"
+    proof(simp only:inv4_A1_def p_2_3_conpred_def R4_A3_def; rule impI)
+      assume "toEnvNum st_final st_final < 10 \<and>
+              getVarBool (predEnv st_final) ''rotation'' \<and>
+              getVarBool st_final ''pressure''"
+      thus "getVarBool st_final ''brake''" using assms by auto
+    qed
+    ultimately show ?thesis using P3_lemma A3_R4 by auto
+  qed
+qed
+
 end
