reflex case stadies/RevolvingDoor/RevolvingDoor_VC8.thy
@@ -122,38 +122,57 @@ next
     qed
   qed
 next
-  show "extra5 st_final" 
-  proof(simp only: extra5_def;rule allI;rule impI)
-    fix s1
-    assume prems:"toEnvP s1 \<and>
-          substate s1 st_final \<and>
-          getPstate s1 ''Controller''=''suspended''"
-    then show "\<exists>s2 s3.
-             toEnvP s2 \<and>
-             toEnvP s3 \<and>
-             substate s2 s3 \<and>
-             substate s3 s1 \<and>
-             toEnvNum s2 s3 = 1 \<and>
-             (getPstate s2 ''Controller'' = ''motionless'' \<and> getVarBool s3 ''user'' \<or>
-              getPstate s2 ''Controller'' = ''rotating'') \<and>
-             getVarBool s3 ''pressure'' \<and>
-             (\<forall>s4. toEnvP s4 \<and> substate s3 s4 \<and> substate s4 s1 \<longrightarrow>
-                   getPstate s4 ''Controller'' = ''suspended'')"
-    proof (cases)
-      assume 1:"s1=st_final"
-      have 2:"substate st0 st_final" using assms substate_refl by auto
-      have 3:"getPstate st0 ''Controller'' = ''suspended''" using assms by auto
-      then have 4:"\<not>(getPstate st0 ''Controller'' = ''motionless'' \<and> getVarBool st_final ''user'' \<or>
-              getPstate st0 ''Controller'' = ''rotating'')" using assms extraInv_def extraSuspendedOut_def by auto
-      have "extra5 st0" using assms extraInv_def by auto
-      then show ?thesis using 1 2 3 4 prems assms inv1_def extraInv_def substate_trans substate_refl extra5_def by sorry 
-    next
-      assume 1:"s1\<noteq>st_final"
-      have "predEnv st_final = st0" using assms extraInv_def by auto
-      then have 2:"substate s1 st0" using 1 assms prems substate_eq_or_predEnv by blast
-      have "extra5 st0" using assms extraInv_def by auto
-      then show ?thesis using 1 2 prems assms extraInv_def extra5_def by auto
+  have prems:"extra5 st0" using assms extraInv_def by simp
+  show "extra5 st_final"
+  proof -
+    have 0:"toEnvP st0 \<and> toEnvP st_final \<and> st0 = predEnv st_final" using assms extraInv_def by auto
+    moreover have "P6_predEnv extra5_A extra5_B extra5_C st0" using assms extraInv_def extra5 P6_bridge by auto
+    moreover have "(AB_comb_before extra5_A (BC_to_BP4 extra5_B extra5_C)) st_final st_final"
+    proof -
+      have 1:"toEnvP st0 \<and> substate st0 st0 \<and> getPstate st0 ''Controller'' = ''suspended''" 
+        using assms extraInv_def substate_refl by auto
+      then obtain s2 s3 where
+       o1:"toEnvP s2 \<and> 
+          toEnvP s3 \<and> 
+          substate s2 s3 \<and> 
+          substate s3 st0 \<and> 
+          toEnvNum s2 s3 = 1 \<and> 
+          (getPstate s2 ''Controller'' = ''motionless'' \<and> 
+            getVarBool s3 ''user'' \<or>
+            getPstate s2 ''Controller'' = ''rotating'') \<and> 
+          getVarBool s3 ''pressure'' \<and>
+          (\<forall> s4. toEnvP s4 \<and> substate s3 s4 \<and> substate s4 st0 \<longrightarrow> 
+              getPstate s4 ''Controller'' = ''suspended'')" using extra5_def prems by blast
+      have 2:"substate st0 st_final" using calculation(1) predEnv_substate by auto
+      then have 3:"substate s3 st_final" using o1 substate_trans by blast
+      define subA where "subA \<equiv> (\<lambda>x. substate s3 x \<longrightarrow> getPstate x ''Controller'' = ''suspended'')"
+      then have "P1 subA st0" using P1_def o1 SMT.verit_bool_simplify(4) by auto
+      moreover have "subA st_final" using assms subA_def by auto
+      ultimately have "P1 subA st_final" using 0 P1_lemma by auto
+      then have 4:"(\<forall>s4. toEnvP s4 \<and> substate s3 s4 \<and> substate s4 st_final \<longrightarrow>
+                getPstate s4 ''Controller'' = ''suspended'')" using P1_def subA_def by auto
+      have 5:"s2 = predEnv s3"using o1 toEnvNum_predEnv by auto
+      have 6:"s2\<noteq>emptyState" using o1 by auto
+      have "(\<exists>s2.
+                  toEnvP s2 \<and> 
+                  substate s2 st_final \<and> 
+                  ((getPstate (predEnv s2) ''Controller'' = ''motionless'' \<and>
+                  getVarBool s2 ''user'' \<or>
+                  getPstate (predEnv s2) ''Controller'' = ''rotating'') \<and>
+                  getVarBool s2 ''pressure'') \<and>
+                  (predEnv s2) \<noteq>emptyState \<and>
+                  (\<forall>s3. toEnvP s3 \<and> substate s2 s3 \<and> substate s3 st_final \<longrightarrow>
+                          getPstate s3 ''Controller'' = ''suspended''))" using o1 3 4 5 6 by blast
+      then show ?thesis
+        apply (simp only:AB_comb_before_def BC_to_BP4_def extra5_A_def extra5_B_def extra5_C_def)
+        using predEnvP_or_emptyState by blast
     qed
+    moreover have "(\<forall>x. toEnvP x \<and> substate x st_final \<and> extra5_A st_final x \<and> \<not> extra5_A st0 x \<longrightarrow> 
+        (\<exists>y. toEnvP y \<and> substate y x \<and> substate y st_final \<and> (BC_to_BP4 extra5_B extra5_C) x y))" 
+      using assms extraInv_def extra5_def BC_to_BP4_def extra5_A_def extra5_B_def extra5_C_def
+      by (smt (verit, best)) 
+    ultimately have "P6_cons extra5_A extra5_B extra5_C st_final" using P6_lemma extra5 prems by blast
+    thus ?thesis using P6_bridge extra5 by auto
   qed
 next
   show "extra7 st_final"
@@ -202,9 +221,9 @@ next
   show "R1 st_final"
   proof -
     have "toEnvP st0 \<and> toEnvP st_final \<and> st0 = predEnv st_final" using assms inv1_def extraInv_def by auto
-    moreover have "P2_predEnv R1_A2 st0" using R1_A2 assms inv1_def by auto
+    moreover have "P2_1_cons R1_A2 st0" using R1_A2 assms inv1_def by auto
     moreover have "R1_A2 st_final st0" using assms R1_A2_def by auto
-    ultimately show ?thesis using two_pos_cond_cons_exp A2_R1 by auto
+    ultimately show ?thesis using P2_1_lemma A2_R1 by auto
   qed
 qed
 
@@ -224,14 +243,14 @@ next
   show "R2 st_final"
   proof -
     have "toEnvP st0 \<and> toEnvP st_final \<and> st0 = predEnv st_final" using assms inv2_def extraInv_def by auto
-    moreover have "P2_predEnv R2_A2 st0" using R2_A2 assms inv2_def by auto
+    moreover have "P2_1_cons R2_A2 st0" using R2_A2 assms inv2_def by auto
     moreover have "R2_A2 st_final st0" using assms R2_A2_def by auto
-    ultimately show ?thesis using two_pos_cond_cons_exp A2_R2 by auto
+    ultimately show ?thesis using P2_1_lemma A2_R2 by auto
   qed
 qed
 
 lemma
- assumes base_inv:"(inv st0)"
+ assumes base_inv:"(inv6 st0)"
  and st1:"(st1=(setVarBool st0 ''pressure'' pressure))"
  and st2:"(st2=(setVarBool st1 ''user'' user))"
  and st2_Controller_state:"(getPstate st2 ''Controller'')=''suspended''"
@@ -239,5 +258,52 @@ lemma
  and st3:"(st3=(reset st2 ''Controller''))"
  and st4:"(st4=(toEnv st3))"
  and st_final:"(st_final=st4)"
-shows "(inv st_final)"
+shows "(inv6 st_final)"
+proof(simp only: inv6_def; rule conjI)
+  show "extraInv st_final" using assms extra inv6_def by auto
+next
+  have extra:"extraInv st_final" using assms extra inv6_def by auto
+  show "R6 st_final"
+  proof -
+    have 0:"toEnvP st0 \<and> toEnvP st_final \<and> st0 = predEnv st_final" using assms R6_def inv6_def by auto
+    moreover have "P1 R6_A st0" using assms inv6_def R6_A by auto
+    moreover have "R6_A st_final" 
+      using R6_A_def assms inv6_def extraInv_def extraSuspendedOut_def extraMotionlessOut_def extraControllerStates_def extraRotatingOut_def local.extra substate_refl
+      by (smt (verit)) 
+    ultimately have "P1 R6_A st_final" using P1_lemma by blast
+    thus ?thesis using A_R6 0 by auto
+  qed
+qed
+
+lemma
+ assumes base_inv:"(inv4 st0)"
+ and st1:"(st1=(setVarBool st0 ''pressure'' pressure))"
+ and st2:"(st2=(setVarBool st1 ''user'' user))"
+ and st2_Controller_state:"(getPstate st2 ''Controller'')=''suspended''"
+ and st2_if8:"(getVarBool st2 ''pressure'')=True"
+ and st3:"(st3=(reset st2 ''Controller''))"
+ and st4:"(st4=(toEnv st3))"
+ and st_final:"(st_final=st4)"
+shows "(inv4 st_final)"
+proof(simp only: inv4_def; rule conjI)
+  show "extraInv st_final" using assms extra inv4_def by auto
+next
+  have extra:"extraInv st_final" using assms extra inv4_def by auto
+  show "R4_full st_final"
+  proof -
+    define inv4_A1 where "inv4_A1 \<equiv> (p_2_3_conpred R4_A3) st_final "
+    moreover have "toEnvP st0 \<and> toEnvP st_final \<and> st0 = predEnv st_final" using assms R4_full_def inv4_def by auto
+    moreover have "P3_cons R4_A3 st0" using assms inv4_def R4_A3 R4_full_def by auto
+    moreover have "P1 inv4_A1 st0"
+    proof(simp only: P1_def p_2_3_conpred_def R4_A3_def inv4_A1_def SMT.verit_bool_simplify(4); rule allI; rule impI)
+      show "getVarBool st_final ''brake''" using assms inv4_def extraInv_def extraSuspendedOut_def substate_refl by auto
+    qed 
+    moreover have "inv4_A1 st_final" 
+    proof(simp only:  p_2_3_conpred_def R4_A3_def inv4_A1_def SMT.verit_bool_simplify(4); rule impI)
+      show "getVarBool st_final ''brake''" using assms inv4_def extraInv_def extraSuspendedOut_def substate_refl by auto
+    qed 
+    ultimately show ?thesis using P3_lemma A3_R4 by auto
+  qed
+qed
+
 end
